+shallow embedding

ClassicalLanguage/ShallowEmbedding/Condition.lean
@@ -4,4 +4,8 @@ import ClassicalLanguage.State.State
 -- logical condition
 def Cond := State → Bool
 
-def fol(c1: Cond)(c2: Cond) := ∀s:State, c1 s → c2 s
+def CondFol(c1: Cond)(c2: Cond):Prop := ∀s:State, c1 s → c2 s
+
+def CondAnd(c1: Cond)(c2: Cond):Cond := (fun s:State => (c1 s) && (c2 s))
+
+def CondNot(c1: Cond):Cond := (fun s:State => ¬(c1 s))
